### Derivation for [Ĵ², Ĵ_z] = 0
Using Leibniz rule [[<5>]]:
$$[\hat{J}_z, \hat{J}_x^2 + \hat{J}_y^2 + \hat{J}_z^2] = [\hat{J}_z, \hat{J}_x^2] + [\hat{J}_z, \hat{J}_y^2] + [\hat{J}_z, \hat{J}_z^2]$$
For the x term:
$$[\hat{J}_z, \hat{J}_x^2] = \hat{J}_x[\hat{J}_z, \hat{J}_x] + [\hat{J}_z, \hat{J}_x]\hat{J}_x = \hat{J}_x(i\hbar\hat{J}_y) + (i\hbar\hat{J}_y)\hat{J}_x$$
For the y term:
$$[\hat{J}_z, \hat{J}_y^2] = \hat{J}_y[\hat{J}_z, \hat{J}_y] + [\hat{J}_z, \hat{J}_y]\hat{J}_y = -\hat{J}_y(i\hbar\hat{J}_x) - (i\hbar\hat{J}_x)\hat{J}_y$$
The z term vanishes: [Ĵ_z, Ĵ²_z] = 0
Combining:
$$i\hbar(\hat{J}_x\hat{J}_y + \hat{J}_y\hat{J}_x - \hat{J}_y\hat{J}_x - \hat{J}_x\hat{J}_y) = 0$$