Rotation must be **unitary** to preserve normalization.
## Unitarity Requirement
Assume form:
$$\hat{R}(d\phi\hat{k}) = \hat{I} - \frac{i}{\hbar}\hat{J} d\phi$$
$$\hat{R}^\dagger\hat{R} = \left(\hat{I} + \frac{i}{\hbar}\hat{J}^\dagger d\phi\right)\left(\hat{I} - \frac{i}{\hbar}\hat{J} d\phi\right)= \hat{I} + \frac{i}{\hbar}(\hat{J}^\dagger - \hat{J})d\phi + O(d\phi^2)$$
For this to equal ÃŽ (drop higher-order terms):
$$\hat{J}^\dagger - \hat{J} = 0 \implies \hat{J}^\dagger = \hat{J}$$
## Related
- [[Rotation Operators]]
- [[Taylor Expansion for Rotation Operator]]