 Start with [[Schr√∂dinger Equation (Time-Dependent)]]: $$i\hbar \frac{d}{dt}\ket{\psi(t)} = \hat{H}\ket{\psi(t)}$$
 Works for any state $\ket{\psi (t)}$
 If you have an energy eigenstate $\ket{E}$, its time evolution is:
 $$\ket{\psi (t)}=e^{-iEt/h}\ket{E}$$
 Plug this into the time-dependent equation:
 $$i\hbar \frac{d}{dt}(e^{-iEt/h}\ket{E}) = \hat{H}(e^{-iEt/h}\ket{E})$$
 Take the time derivative on the left:
 $$i\hbar \cdot\left(-\frac{iE}{\hbar}\right)(e^{-iEt/h}\ket{E}) = \hat{H}(e^{-iEt/h}\ket{E})$$
 That's how we get the time-independent equation:
 $$E\ket{E}=\hat{H}\ket{E}$$
 