 #ket_vector 
$$\ket{\psi} = c_+ \ket{+z}+ c_- \ket{-z}$$
To extract c+ and c-, we project them onto ⟨+z| and ⟨-z|, respectively:
$$\braket{+z|\psi} = \bra{+z} (c_+\ket{+z} + c_-\ket{-z})$$
$$\braket{+z|\psi} = c_+\braket{+z|+z} + c_-\braket{+z|-z} = c_+$$
$$\braket{-z|\psi} = c_+\braket{-z|+z} + c_-\braket{-z|-z} = c_-$$
---
#bra_vector 
$$\bra{\psi} = c_+' \bra{+z}+ c_-' \bra{-z}$$
$$\braket{\psi|+z} = (c_+'\bra{+z} + c_-'\bra{-z})\ket{+z} = c_+'$$
$$\braket{\psi|-z} = (c_+'\bra{+z} + c_-'\bra{-z})\ket{-z} = c_-'$$
---

$$\braket{\psi|\psi} = \braket{\psi|+z}\braket{+z|\psi} + \braket{\psi|-z} \braket{-z|\psi} = 1$$
To satisfy this, we need to have ⟨ψ|+z⟩ = ⟨+z|ψ⟩* and ⟨ψ|-z⟩ = ⟨-z|ψ⟩* (for the outcome to be real)
c'+' = c*+ and c'- = c*- (complex conjugates as well). Therefore:
$$\braket{\psi|\psi} = \braket{+z|\psi}^*\braket{+z|\psi} + \braket{-z|\psi}^* \braket{-z|\psi} = c^*_+c_+ + c^*_-c_-  = 1$$
Or:
$$\braket{\psi|\psi} = |\braket{+z|\psi}|^2 + |\braket{-z|\psi}|^2 = 1$$