Rotation of $\ket{+z}$ about z-axis:
$$d\phi = \lim_{N \to \infty}\frac{\phi}{N}$$
So using Taylor expansion:
$$\hat{R}(\phi k) = \lim_{N\to\infty}\left[ 1 - \frac{i}{\hbar} \hat{J_z}\left( \frac{\phi}{N} \right) \right]^N = e^{-i\hat{J_z}\frac{\phi}{\hbar}}$$
For $\ket{+z}$ state, it's $\hat{J_z}\ket{+z} = \text{(constant)} \ket{+z}$
$$\hat{R}(\phi k)\ket{+z} = \left[ 1 - \frac{i\phi\hat{J_z}}{\hbar} + \frac{1}{2!} \left( \frac{-i\phi\hat{J_z}}{\hbar} \right)^2 + ... \right]\ket{+z}$$
Constant is the eigenvalue. If $\hat{J_z}\ket{+z} \neq \text{(constant)} \ket{+z}$ and constant involves some other axis component, then the whole thing inside the square brackets will yield $\ket{+z}$ plus some term with other kets, which cannot be canceled, since each term with a different power of $\phi$ is linearly independent.
> Thus, it is deduced that $\ket{+z}$ must be an eigenstate of $\hat{J}_z$: $\hat{J}_z\ket{\pm z} = \pm \frac{\hbar}{2}\ket{\pm z}$


$$\hat{R}(\phi k)\ket{+z} = \left[ 1 - \frac{i\phi}{2} + \frac{1}{2!} \left( \frac{-i\phi}{2} \right)^2 + ... \right]\ket{+z} = e^{-\frac{i\phi}{2}} \ket{+z}$$
Picked up an overall phase ($e^{-\frac{i\phi}{2}} \ket{+z}$ and $e^{\frac{i\phi}{2}} \ket{-z}$)