$$\ket{+x} = \frac{e^{i\beta_+}}{\sqrt{2}}\ket{+z} + \frac{e^{i\beta_-}}{\sqrt{2}}\ket{-z} = \frac{e^{i\beta_+}}{\sqrt{2}}\left[ \ket{+z}+r^{i(\beta_- - \beta_+)}\ket{-z} \right]$$
$$\ket{+y} = \frac{e^{i\gamma_+}}{\sqrt{2}}\ket{+z} + \frac{e^{i\gamma_-}}{\sqrt{2}}\ket{-z} = \frac{e^{i\gamma_+}}{\sqrt{2}}\left[ \ket{+z}+r^{i(\gamma_- - \gamma_+)}\ket{-z} \right]$$
Since $\beta - \gamma = \pm\frac{\pi}{2}$, we usually take:
$$\ket{+x} = \frac{1}{\sqrt{2}}\ket{+z} + \frac{1}{\sqrt{2}}\ket{-z}$$
$$\ket{+y} = \frac{1}{\sqrt{2}}\ket{+z} + \frac{i}{\sqrt{2}}\ket{-z}$$
