$$J^\pm =\hbar\sqrt{j(j+1) - m(m\pm1)}\ket{j, m\pm 1}$$
$$\langle j, m' | J^\pm | j, m \rangle = \hbar \sqrt{j(j+1)-m(m\pm 1)} \; \delta_{m', m\pm1}$$
## j = 0
- $\hat{J}_+ = (0)$
- $\hat{J}_- = (0)$
## j =1/2
$J^+ = \hbar \begin{pmatrix} 0 & 1 \\ 0 & 0 \end{pmatrix}, \quad J^- = \hbar \begin{pmatrix} 0 & 0 \\ 1 & 0 \end{pmatrix}$
## j = 1
$$J^+ = \hbar \begin{pmatrix} 0 & \sqrt{2} & 0 \\ 0 & 0 & \sqrt{2} \\ 0 & 0 & 0 \end{pmatrix}, \quad J^- = \hbar \begin{pmatrix} 0 & 0 & 0 \\ \sqrt{2} & 0 & 0 \\ 0 & \sqrt{2} & 0 \end{pmatrix}$$
## j = 3/2
$$J^+ = \hbar \begin{pmatrix} 0 & \sqrt{3} & 0 & 0 \\ 0 & 0 & 2 & 0 \\ 0 & 0 & 0 & \sqrt{3} \\ 0 & 0 & 0 & 0 \end{pmatrix}, \quad J^- = \hbar \begin{pmatrix} 0 & 0 & 0 & 0 \\ \sqrt{3} & 0 & 0 & 0 \\ 0 & 2 & 0 & 0 \\ 0 & 0 & \sqrt{3} & 0 \end{pmatrix}$$
