Using Leibniz rule [[<5>]]:

$$\begin{align*}
[\hat{J}_z, \hat{J}_x^2 + \hat{J}_y^2 + \hat{J}_z^2] 
&= [\hat{J}_z, \hat{J}_x^2] + [\hat{J}_z, \hat{J}_y^2] + [\hat{J}_z, \hat{J}_z^2] \\
&= \hat{J}_x [\hat{J}_z, \hat{J}_x] + [\hat{J}_z, \hat{J}_x]\hat{J}_x 
   + \hat{J}_y [\hat{J}_z, \hat{J}_y] + [\hat{J}_z, \hat{J}_y]\hat{J}_y \\
&= \hat{J}_x \cdot i\hbar \hat{J}_y + i\hbar \hat{J}_y \hat{J}_x 
   - \hat{J}_y \cdot i\hbar \hat{J}_x - i\hbar \hat{J}_x \hat{J}_y \\
&= i\hbar \left(\hat{J}_x \hat{J}_y + \hat{J}_y \hat{J}_x - \hat{J}_y \hat{J}_x - \hat{J}_x \hat{J}_y\right) \\
&= 0
\end{align*}$$
