## Eigenvalue Problem
**Setup:**
$$\hat{S} = \hat{S}_x \hat{i} + \hat{S}_y \hat{j} + \hat{S}_z \hat{k}$$
$$\mathbf{n} = \sin\theta\cos\phi \,\hat{i} + \sin\theta\sin\phi\, \hat{j} + \cos\theta\, \hat{k}$$
$$\hat{S} \cdot \mathbf{n} = \frac{\hbar}{2}\begin{bmatrix} \cos\theta & \sin\theta(\cos\phi - i\sin\phi) \\ \sin\theta(\cos\phi + i\sin\phi) & -\cos\theta \end{bmatrix} = \frac{\hbar}{2}\begin{bmatrix} \cos\theta & \sin\theta\, e^{-i\phi} \\ \sin\theta\, e^{i\phi} & -\cos\theta \end{bmatrix}$$
**Characteristic polynomial:**
$$\det(\hat{S} \cdot \mathbf{n} - \lambda I) = 0$$
$$\frac{\hbar}{2}\left[(\cos\theta - \lambda')(-\cos\theta - \lambda') - \sin^2\theta(\cos\phi - i\sin\phi)(\cos\phi + i\sin\phi)\right] = 0$$
where $\lambda' = \frac{2\lambda}{\hbar}$

$$-\cos^2\theta + \lambda'^2 - \sin^2\theta = 0$$
$$\lambda'^2 = 1 \quad \Rightarrow \quad \lambda = \pm\frac{\hbar}{2}$$
---
## Eigenvector for $\lambda = +\frac{\hbar}{2}$
$$\frac{\hbar}{2}\begin{bmatrix} \cos\theta - 1 & e^{-i\phi}\sin\theta \\ e^{i\phi}\sin\theta & \cos\theta - 1 \end{bmatrix}\begin{bmatrix} v_1 \\ v_2 \end{bmatrix} = 0$$
From first equation:
$$(\cos\theta - 1)v_1 + e^{-i\phi}\sin\theta \, v_2 = 0$$
$$v_2 = \frac{e^{i\phi}(1-\cos\theta)}{\sin\theta} v_1$$
So: $|+n\rangle \sim \begin{bmatrix} 1 \\ \frac{e^{i\phi}(1-\cos\theta)}{\sin\theta} \end{bmatrix}$

**Normalize:**
$$1 + \frac{(1-\cos\theta)^2}{\sin^2\theta} = 1 + \frac{1 - 2\cos\theta + \cos^2\theta}{\sin^2\theta} = \frac{\sin^2\theta + 1 - 2\cos\theta + \cos^2\theta}{\sin^2\theta}$$

$$= \frac{2 - 2\cos\theta}{\sin^2\theta} = \frac{2(1-\cos\theta)}{\sin^2\theta}$$

Using $1 - \cos\theta = 2\sin^2\frac{\theta}{2}$ and $\sin\theta = 2\sin\frac{\theta}{2}\cos\frac{\theta}{2}$:

$$= \frac{4\sin^2\frac{\theta}{2}}{4\sin^2\frac{\theta}{2}\cos^2\frac{\theta}{2}} = \frac{1}{\cos^2\frac{\theta}{2}}$$

Also: $\frac{e^{i\phi}(1-\cos\theta)}{\sin\theta} \cdot \cos\frac{\theta}{2} = \frac{2e^{i\phi}\sin^2\frac{\theta}{2}}{2\sin\frac{\theta}{2}\cos\frac{\theta}{2}} = e^{i\phi}\sin\frac{\theta}{2}$

$$\boxed{\ket{+n} = \cos\frac{\theta}{2}|+z\rangle + e^{i\phi}\sin\frac{\theta}{2}|-z\rangle}$$
---
## Eigenvector for $\lambda = -\frac{\hbar}{2}$
$$\begin{bmatrix} \cos\theta + 1 & e^{-i\phi}\sin\theta \\ e^{i\phi}\sin\theta & \cos\theta + 1 \end{bmatrix}\begin{bmatrix} v_1 \\ v_2 \end{bmatrix} = 0$$
$$(\cos\theta + 1)v_1 + e^{-i\phi}\sin\theta \, v_2 = 0$$
$$v_2 = \frac{-(cos\theta + 1)e^{i\phi}}{\sin\theta} v_1$$
So: $|-n\rangle \sim \begin{bmatrix} 1 \\ \frac{-(\cos\theta+1)e^{i\phi}}{\sin\theta} \end{bmatrix}$
**Normalize:**
$$1 + \frac{(\cos\theta+1)^2}{\sin^2\theta} = 1 + \frac{\cos^2\theta + 2\cos\theta + 1}{\sin^2\theta} = \frac{2 + 2\cos\theta}{\sin^2\theta} = \frac{2(1+\cos\theta)}{\sin^2\theta}$$
Using $1 + \cos\theta = 2\cos^2\frac{\theta}{2}$:
$$= \frac{4\cos^2\frac{\theta}{2}}{4\sin^2\frac{\theta}{2}\cos^2\frac{\theta}{2}} = \frac{1}{\sin^2\frac{\theta}{2}}$$

$$\boxed{\ket{-n} = \sin\frac{\theta}{2}|+z\rangle - e^{i\phi}\cos\frac{\theta}{2}|-z\rangle}$$