## Derive $\hat{J}_-|j,m\rangle = \sqrt{j(j+1)-m(m-1)}\hbar|j,m-1\rangle$

$$\hat{J}_+|j,m\rangle = c_+\hbar|j,m+1\rangle \qquad \hat{J}_-|j,m\rangle = c_-\hbar|j,m-1\rangle$$

Start with the inner product with $\hat{J}_+$ (which is the same thing as $\hat{J}^\dagger_-$):

$$\langle j,m|\hat{J}_+\hat{J}_-|j,m\rangle = c_+^* c_-\hbar^2\langle j,m-1|j,m-1\rangle$$
$$\hat{J}_+\hat{J}_- = (\hat J_x + i \hat J_y)(\hat J_x - i \hat J_y) = \hat J_x^2 + \hat J_y^2 -i[\hat J_x, \hat J_y] = \hat{J}^2 - \hat{J}_z^2 + \hbar\hat{J}_z$$
$$\langle j,m|\hat{J}^2 - \hat{J}_z^2 + \hbar\hat{J}_z|j,m\rangle = [j(j+1) - m^2 + m]\hbar^2 = c_-^* c_-\hbar^2\langle j,m-1|j,m-1\rangle$$

Assuming $\langle j,m|j,m\rangle = \langle j,m-1|j,m-1\rangle$:
$$\hat{J}_-|j,m\rangle = \sqrt{j(j+1)-m^2+m}\hbar|j,m-1\rangle = \sqrt{j(j+1)-m(m-1)}\hbar|j,m-1\rangle$$